

## Extra: Algebra for the Lifetime BC

$$W_{b+1} = y_{b+1} + (1+r)(W_b - C_t) \Rightarrow W_b = \frac{W_{b+1} - y_{b+1}}{1+r} + C_b$$

Subs  $W_{b+1} = \frac{W_{b+2} - y_{b+2}}{1+r} + C_{b+1}$  in the budget constraint:

$$\frac{W_{b+2} - y_{b+2}}{1+r} + C_{b+1} = y_{b+1} + (1+r)(W_b - C_b)$$

Subs  $W_{b+2}$ :

$$\frac{W_{b+3} - y_{b+3}}{(1+r)^2} + \frac{C_{b+2}}{1+r} - \frac{y_{b+2}}{1+r} + C_{b+1} = y_{b+1} + (1+r)(W_b - C_b)$$

$$\Rightarrow \frac{W_{b+3}}{(1+r)^2} + (1+r)C_b + C_{b+1} + \frac{C_{b+2}}{1+r} = y_{b+1} + \frac{y_{b+2}}{1+r} + \frac{y_{b+3}}{(1+r)^2} + (1+r)W_b$$

Subs  $W_{b+3}$ :

$$\frac{W_{b+4} - y_{b+4}}{(1+r)^3} + \frac{C_{b+3}}{(1+r)^2} + (1+r)C_b + C_{b+1} + \frac{C_{b+2}}{1+r} = y_{b+1} + \frac{y_{b+2}}{1+r} + \frac{y_{b+3}}{(1+r)^2} + (1+r)W_b$$

$$\text{or } \frac{W_{b+4}}{(1+r)^3} + (1+r)C_b + C_{b+1} + \frac{C_{b+2}}{1+r} + \frac{C_{b+3}}{(1+r)^2} = y_{b+1} + \frac{y_{b+2}}{1+r} + \frac{y_{b+3}}{(1+r)^2} + \frac{y_{b+4}}{(1+r)^3} + (1+r)W_b$$

this equation holds for every period and we'll use it to substitute forward the terms  $W_{b+1}, W_{b+2}, W_{b+3}, W_{b+4}, \dots$

Subs  $W_{b+4}$ :

$$(1+r)C_b + C_{b+1} + \frac{C_{b+2}}{1+r} + \frac{C_{b+3}}{(1+r)^2} + \frac{C_{b+4}}{(1+r)^3} = (1+r)W_b + y_{b+1} + \frac{y_{b+2}}{1+r} + \frac{y_{b+3}}{(1+r)^2} + \frac{y_{b+4}}{(1+r)^3} + \frac{y_{b+5}}{(1+r)^4}$$

$$\Rightarrow C_b + \frac{C_{b+1}}{1+r} + \frac{C_{b+2}}{(1+r)^2} + \frac{C_{b+3}}{(1+r)^3} + \frac{C_{b+4}}{(1+r)^4} = W_b + \frac{y_{b+1}}{1+r} + \frac{y_{b+2}}{(1+r)^2} + \frac{y_{b+3}}{(1+r)^3} + \frac{y_{b+4}}{(1+r)^4} + \frac{y_{b+5}}{(1+r)^5}$$

•  
• So on,  
•

$$\sum_{s=0}^{\infty} \left(\frac{1}{1+r}\right)^s C_{b+s} = W_b + \sum_{s=0}^{\infty} \left(\frac{1}{1+r}\right)^s y_{b+s}$$

Take  $t=0$  (could do this for any  $t=1, 2, \dots$ )

$$\Rightarrow \sum_{s=0}^{\infty} \left(\frac{1}{1+r}\right)^s C_s = W_0 + \sum_{s=0}^{\infty} \left(\frac{1}{1+r}\right)^s y_s \quad (\text{as in the lecture})$$

More detailed algebra steps (CAPM from Euler Eq)

$$E_t \left\{ \frac{u'(C_{t+1})}{u'(C_t)} \frac{(1+\tilde{r}_t^i)}{1+p} \right\} = 1 \quad \forall i, \quad M_t = \frac{u'(C_{t+1})}{u'(C_t)} \frac{1}{1+p} \equiv \text{Stochastic discount Factor}$$

(  $\beta = \frac{1}{1+p} \equiv \frac{\text{Standard discount}}{\text{Factor}}$  )

$$\Rightarrow E_t \{ \tilde{M}_t (1+\tilde{r}_t^i) \} = 1 \Rightarrow E_t(\tilde{M}_t) E_t(1+\tilde{r}_t^i) + \text{Cov}(1+\tilde{r}_t^i, \tilde{M}_t) = 1 \quad \left( \begin{array}{l} \text{uses that:} \\ \text{Cov}(X,Y) = E(XY) - E(X)E(Y) \end{array} \right)$$

With CRRA:  $\tilde{M}_t = \beta \left( \frac{C_{t+1}}{C_t} \right)^{-\gamma}$

$$\Rightarrow E_t(1+\tilde{r}_t^i) = \frac{1}{E_t(\tilde{M}_t)} \left[ 1 - \beta \text{Cov}(1+\tilde{r}_t^i, \left( \frac{C_{t+1}}{C_t} \right)^{-\gamma}) \right]$$

use that  $\frac{C_{t+1}}{C_t} \approx 1 + \Delta \ln C_{t+1}$  (i)  $\frac{X_{t+1}}{X_t} \approx 1 + \% \text{growth in } X \approx (1+g_x)$ . (ii)  $\ln(1+g_x) \approx g_x$ . (iii) Percentage growth  $\equiv g_x \approx \ln X_{t+1} - \ln X_t = \Delta \ln X_{t+1}$

$$E_t(1+\tilde{r}_t^i) = \frac{1}{E_t(\tilde{M}_t)} \left[ 1 - \beta \text{Cov}(1+\tilde{r}_t^i, (1+\Delta \ln C_{t+1})^{-\gamma}) \right]$$

$$= \frac{1}{E_t(\tilde{M}_t)} \left[ 1 - \beta \text{Cov}(1+\tilde{r}_t^i, 1 - \gamma \Delta \ln C_{t+1}) \right]$$

Uses binomial approximation:  $(1+x)^\alpha \approx 1 + \alpha x$

$$= \frac{1}{1+p} \frac{1}{E_t(\tilde{M}_t)} \left[ 1+p - \text{Cov}(\tilde{r}_t^i, -\gamma \Delta \ln C_{t+1}) \right] = \frac{1}{(1+p)E_t(\tilde{M}_t)} \left\{ 1+p + \gamma \text{Cov}(\tilde{r}_t^i, \Delta \ln C_{t+1}) \right\}$$

Algebra for log-linearizing Euler Equation.

Depart from Euler Equation:  $C_b^{-\gamma} = \beta E_b [C_{b+1}^{-\gamma} R_{b+1}]$

Assume RHS variables are jointly log-normal & homoskedastic

Take logs:  $-\gamma \log C_b = \log \beta + \log E_b [C_{b+1}^{-\gamma} R_{b+1}]$

w/ log normality:  $\log(E_b(X_{b+1})) = E_b[\log(X_{b+1})] + \frac{1}{2} \text{Var}_b[\log(X_{b+1})]$

$$\Rightarrow \log E_b [C_{b+1}^{-\gamma} R_{b+1}] = E_b [\log (C_{b+1}^{-\gamma} R_{b+1})] + \frac{1}{2} \text{Var}_b [\log (C_{b+1}^{-\gamma} R_{b+1})]$$

$$= -\gamma E_b \log C_{b+1} + E_b \log R_{b+1} + \frac{\gamma^2}{2} \sigma_{E, \log C_{b+1}}^2 + \frac{1}{2} \sigma_{b, \log R_{b+1}}^2 - \gamma \sigma_{b, \log C_{b+1}, \log R_{b+1}}$$

$$\Rightarrow -\gamma \log C_b = \log \beta + E_b (-\gamma \log C_{b+1} + \log R_{b+1}) + \underbrace{\frac{\gamma^2}{2} \sigma_{b, \log C_{b+1}}^2 + \frac{1}{2} \sigma_{b, \log R_{b+1}}^2 - \gamma \sigma_{b, \log C_{b+1}, \log R_{b+1}}}_{\text{Constant}}$$

Subtract Equation for Steady State

$$-\gamma d \log C_b = -\gamma E_b d \log C_{b+1} + E_b d \log R_{b+1}$$

$$d \log Z_b = \hat{Z}_b = \frac{Z_b - Z^{ss}}{Z^{ss}} \quad \left( r_{b+1} = \frac{R_{b+1} - R^{ss}}{R^{ss}} \right)$$

$$\Rightarrow -\gamma \hat{C}_b = -\gamma E_b \hat{C}_{b+1} + E_b r_{b+1}$$

$$\hat{C}_b = E_b \hat{C}_{b+1} - \frac{1}{\gamma} E_b r_{b+1}$$